De_Bruijn/dbmonad.ml
@@ -1,0 +1,305 @@
+(* ========================================================================= *)
+(*  De Bruijn monads and modules.                                            *)
+(*                                                                           *)
+(*  Author: Marco Maggesi                                                    *)
+(*          University of Florence, Italy                                    *)
+(*          http://www.math.unifi.it/~maggesi/                               *)
+(*                                                                           *)
+(*          (c) Copyright, Marco Maggesi 2005 2006 2017, 2020, 2021          *)
+(* ========================================================================= *)
+
+(* ------------------------------------------------------------------------- *)
+(* De Bruijn monads.                                                         *)
+(* ------------------------------------------------------------------------- *)
+
+let MONAD_DEF = new_definition
+  `!op:(num->A)->A->A.
+     MONAD op <=>
+     (!f g x. op g (op f x) = op (\n. op g (f n)) x) /\
+     (?i. (!f n. op f (i n) = f n) /\ (!x. op i x = x))`;;
+
+let UNIT = new_definition
+  `!op:(num->A)->A->A.
+     UNIT op = (@i. (!f n. op f (i n) = f n) /\ (!x. op i x = x))`;;
+
+let MONAD = prove
+ (`!op. MONAD op <=>
+        (!f g x:A. op g (op f x) = op (\n. op g (f n)) x) /\
+        (!f n. op f (UNIT op n) = f n) /\
+        (!x. op (UNIT op) x = x)`,
+  REWRITE_TAC[MONAD_DEF; UNIT] THEN MESON_TAC[]);;
+
+let MONAD_ASSOC = prove
+ (`!op. MONAD op ==> !f g x:A. op g (op f x) = op (op g o f) x`,
+  REWRITE_TAC[MONAD; o_DEF] THEN MESON_TAC[]);;
+
+let MONAD_RUNIT = prove
+ (`!op. MONAD op ==> (!f n. op f (UNIT op n) = f n:A)`,
+  REWRITE_TAC[MONAD] THEN MESON_TAC[]);;
+
+let MONAD_LUNIT = prove
+ (`!op. MONAD op ==> (!x:A. op (UNIT op) x = x)`,
+  REWRITE_TAC[MONAD] THEN MESON_TAC[]);;
+
+let MONAD_LUNIT_IMP = prove
+ (`!op f x:A. MONAD op /\ (!i. f i = UNIT op i) ==> op f x = x`,
+  REPEAT GEN_TAC THEN REWRITE_TAC[GSYM FUN_EQ_THM; ETA_AX] THEN
+  SIMP_TAC[MONAD_LUNIT]);;
+
+let UNIT_UNIQUE = prove
+ (`!op i. MONAD op /\ (!f n. op f (i n) = f n:A) /\ (!x. op i x = x)
+          ==> UNIT op = i`,
+  REWRITE_TAC[MONAD_DEF; UNIT; FUN_EQ_THM] THEN MESON_TAC[]);;
+
+(* ------------------------------------------------------------------------- *)
+(* Reindexing: functoriality of De Bruijn monads.                            *)
+(* ------------------------------------------------------------------------- *)
+
+let FMAP = new_definition
+  `FMAP op f x:A = op (UNIT op o f) x`;;
+
+let FMAP_FMAP = prove
+ (`!op f g x:A.
+     MONAD op
+     ==> FMAP op g (FMAP op f x) = FMAP op (g o f) x`,
+  REPEAT GEN_TAC THEN DISCH_TAC THEN REWRITE_TAC[FMAP] THEN
+  ASM_SIMP_TAC[MONAD_ASSOC] THEN AP_THM_TAC THEN AP_TERM_TAC THEN
+  ASM_SIMP_TAC[MONAD_RUNIT; FUN_EQ_THM; o_THM]);;
+
+let FMAP_UNIT = prove
+ (`!op f i. MONAD op ==> FMAP op f (UNIT op i) = UNIT op (f i):A`,
+  REPEAT GEN_TAC THEN DISCH_TAC THEN REWRITE_TAC[FMAP] THEN
+  ASM_SIMP_TAC[MONAD_RUNIT] THEN REWRITE_TAC[o_THM]);;
+
+let FMAP_OP = prove
+ (`!op f g x:A. MONAD op
+                ==> FMAP op f (op g x) = op (FMAP op f o g) x`,
+  REPEAT GEN_TAC THEN DISCH_TAC THEN
+  ASM_SIMP_TAC[FMAP; MONAD_ASSOC; o_THM] THEN
+  AP_THM_TAC THEN AP_TERM_TAC THEN REWRITE_TAC[FUN_EQ_THM; o_THM; FMAP]);;
+
+let OP_FMAP = prove
+ (`!op f g x:A. MONAD op ==> op f (FMAP op g x) = op (f o g) x`,
+  REPEAT GEN_TAC THEN DISCH_TAC THEN REWRITE_TAC[FMAP] THEN
+  ASM_SIMP_TAC[MONAD_ASSOC] THEN AP_THM_TAC THEN AP_TERM_TAC THEN
+  REWRITE_TAC[FUN_EQ_THM; o_THM] THEN GEN_TAC THEN ASM_SIMP_TAC[MONAD_RUNIT]);;
+
+(* ------------------------------------------------------------------------- *)
+(* Morphisms of De Bruijn monads.                                            *)
+(* ------------------------------------------------------------------------- *)
+
+let MONAD_HOM = define
+  `MONAD_HOM (op1,op2) =
+   {h:A->B | MONAD op1 /\ MONAD op2 /\
+             (!n. h (UNIT op1 n) = UNIT op2 n) /\
+             (!f x. h (op1 f x) = op2 (h o f) (h x))}`;;
+
+let IN_MONAD_HOM = prove
+ (`!op1 op2 h:A->B.
+     h IN MONAD_HOM (op1,op2) <=>
+     MONAD op1 /\ MONAD op2 /\
+     (!n. h (UNIT op1 n) = UNIT op2 n) /\
+     (!f x. h (op1 f x) = op2 (h o f) (h x))`,
+  REWRITE_TAC[MONAD_HOM; IN_ELIM_THM]);;
+
+let MONAD_HOM_ID = prove
+ (`!op:(num->A)->A->A. MONAD op ==> I IN MONAD_HOM (op,op)`,
+  REWRITE_TAC[IN_MONAD_HOM; I_THM; I_O_ID]);;
+
+let MONAD_HOM_o = prove
+ (`!op1 op2 op3 h:A->B g:B->C.
+     h IN MONAD_HOM (op1,op2) /\ g IN MONAD_HOM (op2,op3)
+     ==> g o h IN MONAD_HOM (op1,op3)`,
+  REPEAT GEN_TAC THEN REWRITE_TAC[IN_MONAD_HOM] THEN STRIP_TAC THEN
+  ASM_REWRITE_TAC[o_THM; o_ASSOC]);;
+
+(* ------------------------------------------------------------------------- *)
+(* Modules over De Bruijn monads                                             *)
+(* ------------------------------------------------------------------------- *)
+
+let MODULE = new_definition
+  `MODULE (op:(num->A)->A->A) =
+   {mop:(num->A)->B->B | MONAD op /\
+                         (!x. mop (UNIT op) x = x) /\
+                         (!f g x. mop g (mop f x) = mop (op g o f) x)}`;;
+
+let IN_MODULE = prove
+ (`mop:(num->A)->B->B IN MODULE (op:(num->A)->A->A) <=>
+   MONAD op /\
+   (!x. mop (UNIT op) x = x) /\
+   (!f g x. mop g (mop f x) = mop (op g o f) x)`,
+  REWRITE_TAC[MODULE; IN_ELIM_THM]);;
+
+let MMAP = new_definition
+  `MMAP (op,mop:(num->A)->B->B) f = mop (UNIT op o f)`;;
+
+(* ------------------------------------------------------------------------- *)
+(* Tautological module over a De Bruijn monad.                               *)
+(* ------------------------------------------------------------------------- *)
+
+let SELF_MODULE = prove
+ (`!op:(num->A)->A->A. op IN MODULE op <=> MONAD op`,
+  REWRITE_TAC[MONAD; IN_MODULE; o_DEF] THEN MESON_TAC[]);;
+
+let SELF_FMAP = prove
+ (`!op:(num->A)->A->A. FMAP op = MMAP (op,op)`,
+  REWRITE_TAC[FUN_EQ_THM; FMAP; MMAP]);;
+
+(* ------------------------------------------------------------------------- *)
+(* Product of modules.                                                       *)
+(* ------------------------------------------------------------------------- *)
+
+let MPROD = new_definition
+  `MPROD (mop1:(num->A)->B->B) (mop2:(num->A)->C->C)
+           (f:num->A) (x:B,y:C) : B#C = mop1 f x,mop2 f y`;;
+
+let MPROD_IN_MODULE = prove
+ (`!op mod1:(num->A)->B->B mod2:(num->A)->C->C.
+     mod1 IN MODULE op /\ mod2 IN MODULE op
+     ==> MPROD mod1 mod2 IN MODULE op`,
+  REPEAT GEN_TAC THEN REWRITE_TAC[IN_MODULE] THEN STRIP_TAC THEN
+  ASM_REWRITE_TAC[FORALL_PAIR_THM; MPROD]);;
+
+let MMAP_MPROD = prove
+ (`!op:(num->A)->A->A f x:B y:C.
+     MMAP (op,MPROD mop1 mop2) f (x,y) =
+     MMAP (op,mop1) f x, MMAP (op,mop2) f y`,
+  REWRITE_TAC[MMAP; MPROD]);;
+
+(* ------------------------------------------------------------------------- *)
+(* Morphisms of modules over the same De Bruijn monad.                       *)
+(* ------------------------------------------------------------------------- *)
+
+let MODULE_MOR = new_definition
+  `MODULE_MOR op (mop1,mop2) =
+   {h:B->C | mop1 IN MODULE op /\
+             mop2 IN MODULE op /\
+             (!f:num->A x. h (mop1 f x) = mop2 f (h x))}`;;
+
+let IN_MODULE_MOR = prove
+ (`!op mop1 mop2 h:B->C.
+     h IN MODULE_MOR op (mop1,mop2) <=>
+     mop1 IN MODULE op /\
+     mop2 IN MODULE op /\
+     (!f:num->A x. h (mop1 f x) = mop2 f (h x))`,
+  REWRITE_TAC[MODULE_MOR; IN_ELIM_THM]);;
+
+let MODULE_MOR_MMAP = prove
+ (`!op:(num->A)->A->A mop1 mop2 h:B->C f x.
+     h IN MODULE_MOR op (mop1,mop2)
+     ==> h (MMAP (op,mop1) f x) = MMAP (op,mop2) f (h x)`,
+  REPEAT GEN_TAC THEN REWRITE_TAC[IN_MODULE_MOR] THEN STRIP_TAC THEN
+  ASM_REWRITE_TAC[MMAP]);;
+
+let MODULE_MOR_ID = prove
+ (`!op mop:(num->A)->B->B.
+     I IN MODULE_MOR op (mop,mop) <=> mop IN MODULE op`,
+  REWRITE_TAC[IN_MODULE_MOR; I_THM]);;
+
+let MODULE_MOR_o = prove
+ (`!op:(num->A)->A->A mop1 mop2 g:N->L h:M->N.
+     h IN MODULE_MOR op (mop1,mop2) /\
+     g IN MODULE_MOR op (mop2,mop3)
+     ==> g o h IN MODULE_MOR op (mop1,mop3)`,
+  REWRITE_TAC[IN_MODULE_MOR] THEN REPEAT STRIP_TAC THEN
+  ASM_REWRITE_TAC[o_DEF]);;
+
+(* ------------------------------------------------------------------------- *)
+(* Pull-back module along a module morphism.                                 *)
+(* ------------------------------------------------------------------------- *)
+
+let PBMOP = new_definition
+  `!h:A'->A mop:(num->A)->M->M f.
+     PBMOP h mop f = mop (h o f)`;;
+
+let PB_MODULE = prove
+ (`!op' op h:A'->A mop:(num->A)->M->M.
+      h IN MONAD_HOM (op',op) /\ mop IN MODULE op
+      ==> PBMOP h mop IN MODULE op'`,
+  REWRITE_TAC[IN_MONAD_HOM; IN_MODULE; PBMOP] THEN REPEAT STRIP_TAC THEN
+  ASM_REWRITE_TAC[o_DEF; ETA_AX]);;
+
+(* ------------------------------------------------------------------------- *)
+(* Derived module.                                                           *)
+(* ------------------------------------------------------------------------- *)
+
+let MDERIV = new_recursive_definition num_RECURSION
+  `(!op f. MDERIV op f 0 = UNIT op 0:A) /\
+   (!op f i. MDERIV op f (SUC i) = FMAP op SUC (f i))`;;
+
+let MDERIV_UNIT = prove
+ (`!op. MONAD op ==> MDERIV op (UNIT op) = UNIT op:num->A`,
+  GEN_TAC THEN DISCH_TAC THEN REWRITE_TAC[FUN_EQ_THM] THEN NUM_CASES_TAC THEN
+  REWRITE_TAC[MDERIV] THEN ASM_SIMP_TAC[FMAP_UNIT]);;
+
+let DMOP = new_definition
+  `!op:(num->A)->A->A mop:(num->A)->M->M f:num->A x:M.
+     DMOP op mop f x = mop (MDERIV op f) x:M`;;
+
+let MODULE_DMOP = prove
+ (`!op mop:(num->A)->M->M.
+     mop IN MODULE op ==> DMOP op mop IN MODULE op`,
+  REPEAT GEN_TAC THEN INTRO_TAC "mod" THEN
+  HYP_TAC "mod -> mnd munit massoc" (REWRITE_RULE[IN_MODULE]) THEN
+  ASM_REWRITE_TAC[IN_MODULE] THEN REPEAT STRIP_TAC THEN
+  REWRITE_TAC[DMOP] THEN ASM_SIMP_TAC[MDERIV_UNIT] THEN
+  REWRITE_TAC[o_THM] THEN AP_THM_TAC THEN AP_TERM_TAC THEN
+  REWRITE_TAC[FUN_EQ_THM] THEN NUM_CASES_TAC THEN
+  ASM_SIMP_TAC[MDERIV; MONAD_RUNIT; o_THM; OP_FMAP; FMAP_OP] THEN
+  AP_THM_TAC THEN AP_TERM_TAC THEN REWRITE_TAC[FUN_EQ_THM; o_THM; MDERIV]);;
+
+let DMOP_IN_MODULE_MOR = prove
+ (`!op:(num->A)->A->A mop1 mop2 h:M->N.
+     h IN MODULE_MOR op (mop1,mop2)
+     ==> h IN MODULE_MOR op (DMOP op mop1,DMOP op mop2)`,
+  SIMP_TAC[IN_MODULE_MOR; MODULE_DMOP; DMOP]);;
+
+(* ------------------------------------------------------------------------- *)
+(* Isomorphisms of modules over a De Bruijn monad.                           *)
+(* ------------------------------------------------------------------------- *)
+
+let MODULE_MOR_INV = prove
+ (`!op:(num->A)->A->A mop1 mop2 g:M->N h:N->M.
+     h IN MODULE_MOR op (mop1,mop2) /\
+     (!x. g (h x) = x) /\ (!y. h (g y) = y)
+     ==> g IN MODULE_MOR op (mop2,mop1)`,
+  REWRITE_TAC[IN_MODULE_MOR] THEN MESON_TAC[]);;
+
+let MODULE_ISOM = new_definition
+  `!op:(num->A)->A->A mop1 mop2 h:M->N g:N->M.
+     MODULE_ISOM op (mop1,mop2) (h,g) <=>
+       h IN MODULE_MOR op (mop1,mop2) /\
+       (!x. g (h x) = x) /\ (!y. h (g y) = y)`;;
+
+let MODULE_ISOM_SYM = prove
+ (`!op:(num->A)->A->A mop1 mop2 h:M->N g:N->M.
+     MODULE_ISOM op (mop1,mop2) (h,g)
+     ==> MODULE_ISOM op (mop2,mop1) (g,h)`,
+  REWRITE_TAC[MODULE_ISOM] THEN REPEAT STRIP_TAC THEN ASM_REWRITE_TAC[] THEN
+  MATCH_MP_TAC MODULE_MOR_INV THEN ASM_MESON_TAC[]);;
+
+let MODULE_ISOM_UNFOLD = prove
+ (`!op:(num->A)->A->A mop1 mop2 h:M->N g.
+     MODULE_ISOM op (mop1,mop2) (h,g) <=>
+     mop1 IN MODULE op /\
+     mop2 IN MODULE op /\
+     h IN MODULE_MOR op (mop1,mop2) /\
+     g IN MODULE_MOR op (mop2,mop1) /\
+     (!x. g (h x) = x) /\ (!y. h (g y) = y)`,
+  REPEAT GEN_TAC THEN EQ_TAC THEN STRIP_TAC THENL
+  [ALL_TAC; ASM_REWRITE_TAC[MODULE_ISOM]] THEN
+  FIRST_ASSUM (ASSUME_TAC o MATCH_MP MODULE_ISOM_SYM) THEN
+  RULE_ASSUM_TAC (REWRITE_RULE [MODULE_ISOM]) THEN ASM_REWRITE_TAC[] THEN
+  RULE_ASSUM_TAC (REWRITE_RULE [IN_MODULE_MOR]) THEN ASM_REWRITE_TAC[]);;
+
+let EXP_MONAD = new_definition
+  `!op:(num->A)->A->A h g.
+     EXP_MONAD op h g <=> MODULE_ISOM op (op,DMOP op op) (h,g)`;;
+
+let EXP_MONAD_HOM = new_definition
+  `!op1 h1 g1 op2 h2 g2 f:A->B.
+     EXP_MONAD_HOM op1 h1 g1 op2 h2 g2 f <=>
+     EXP_MONAD op1 h1 g1 /\
+     EXP_MONAD op2 h2 g2 /\
+     f IN MONAD_HOM (op1,op2) /\
+      (!x. h2 (f x) = f (h1 x))`;;
